Client4 + Client5 + SpinlockClient + SpinlockSpec

src/example/Client05.v
@@ -6,7 +6,7 @@ From Fairness Require Import FairBeh Mod Concurrency Linking.
 From Fairness Require Import PCM IProp IPM IPropAux.
 From Fairness Require Import IndexedInvariants OpticsInterp SimWeakest SimWeakestAdequacy.
 From Fairness Require Import TemporalLogic SCMemSpec.
-From Fairness Require Import Spinlock SpinlockSpec SpinlockSpec1 AuthExclsRA ExclsRA OneShotsRA.
+From Fairness Require Import Spinlock SpinlockSpec0 AuthExclsRA ExclsRA OneShotsRA.
 
 Module Client05.
 
@@ -105,10 +105,10 @@ Section SPEC.
   Context {TLRAS : TLRAs STT Γ Σ}.
 
   Context {HasMEMRA: @GRA.inG memRA Γ}.
-  Context {HasAuthExcls : @GRA.inG (AuthExcls.t nat) Γ}.
+  (* Context {HasAuthExcls : @GRA.inG (AuthExcls.t nat) Γ}. *)
   Context {HasOneShots : @GRA.inG (OneShots.t unit) Γ}.
   Context {HasAuthExcls2 : @GRA.inG (AuthExcls.t (nat * nat)) Γ}.
-  Context {HasExcls : @GRA.inG (Excls.t unit) Γ}.
+  (* Context {HasExcls : @GRA.inG (Excls.t unit) Γ}. *)
 
   Ltac red_tl_all := red_tl; red_tl_memra; red_tl_authexcls; red_tl_excls; red_tl_oneshots.
 
@@ -116,39 +116,39 @@ Section SPEC.
 
   (* Namespace for Client05 invariants. *)
   Definition N_Client05 : namespace := (nroot .@ "Client05").
-  Definition N_t2_write : namespace := (nroot .@ "t2_write").
+  (* Definition N_t2_write : namespace := (nroot .@ "t2_write"). *)
+  Context (spinlockN : namespace) `{DISJ: (↑N_state_tgt :coPset) ## (↑spinlockN : coPset)}.
 
   Lemma mask_disjoint_N_Client05_state_tgt : (↑N_Client05 : coPset) ## (↑N_state_tgt : coPset).
   Proof. apply ndot_ne_disjoint. ss. Qed.
-  Lemma mask_disjoint_N_t2_write_state_tgt : (↑N_t2_write : coPset) ## (↑N_state_tgt : coPset).
+  (* Lemma mask_disjoint_N_t2_write_state_tgt : (↑N_t2_write : coPset) ## (↑N_state_tgt : coPset).
   Proof. apply ndot_ne_disjoint. ss. Qed.
   Lemma mask_disjoint_N_Client05_N_t2_write : (↑N_Client05 : coPset) ## (↑N_t2_write : coPset).
-  Proof. apply ndot_ne_disjoint. ss. Qed.
+  Proof. apply ndot_ne_disjoint. ss. Qed. *)
 
-  Definition t2_write n : sProp n :=
-    syn_inv n N_t2_write (D ↦ 1)%S.
+  (* Definition t2_write n : sProp n :=
+    syn_inv n N_t2_write (D ↦ 1)%S. *)
 
-  Global Instance t2_write_persistent n : Persistent (⟦t2_write n, n⟧).
+  (* Global Instance t2_write_persistent n : Persistent (⟦t2_write n, n⟧).
   Proof.
     unfold Persistent. iIntros "H". unfold t2_write. rewrite red_syn_inv.
     iDestruct "H" as "#H". auto.
-  Qed.
+  Qed. *)
 
-  Definition client05Inv γw kw n : sProp n :=
-    (◆[kw, 4] ∗ (((△ γw (1/2)) ∗ (D ↦ 0)) -U-[kw](3)-◇ ((▿ γw tt) ∗ t2_write n)))%S.
+  Definition client05Inv n γw : sProp n := (((△ γw (1/2)) ∗ (D ↦ 0)) ∨ ((▿ γw tt) ∗ (D ↦ 1)))%S.
 
   (** Simulation proof. *)
   Lemma Client05_thread1_spec
         tid n
     :
-    ⊢ ⟦(∀ (γw kw γL γe γs : τ{nat, 1+n}),
-           ((⤉ syn_inv n N_Client05 (client05Inv γw kw n))
+    ⊢ ⟦(∀ (γw κw γL : τ{nat, 1+n}),
+           ((⤉ syn_inv n N_Client05 (client05Inv n γw))
               ∗ (syn_tgt_interp_as n sndl (fun m => (s_memory_black m)))
-              ∗ (⤉ isSpinlock n L γL γe kw 4)
-              ∗ (⤉ isSpinlockUse1 n kw γs γL emp 2)
+              ∗ (⤉ isSpinlock spinlockN n κw L γL emp 3 3)
               ∗ TID(tid)
-              ∗ ◇[kw](3, 1)
-              ∗ (⤉ Duty(tid) []))
+              ∗ ◇[κw](2, 1)
+              ∗ (⤉ Duty(tid) [])
+              ∗ (⤉ -[κw](2)-◇ (▿ γw tt)))
              -∗
              syn_wpsim (S n) tid ⊤
              (fun rs rt => (⤉ (syn_term_cond n tid _ rs rt))%S)
@@ -156,17 +156,24 @@ Section SPEC.
              (fn2th Client05Spec.module "thread1" (tt ↑))
              (fn2th Client05.module "thread1" (tt ↑)))%S, 1+n⟧.
   Proof.
-    iIntros. red_tl. iIntros "%γw". red_tl. iIntros "%kw".
-    red_tl. iIntros "%γL". red_tl. iIntros "%γe". red_tl. iIntros "%γs".
+    iIntros. red_tl. iIntros "%γw". red_tl. iIntros "%κw". red_tl. iIntros "%γL".
     red_tl_all; simpl. rewrite red_syn_inv; rewrite red_syn_tgt_interp_as; rewrite red_syn_wpsim.
 
-    iIntros "(#INV & #MEM & #SPIN & #SPIN1 & TID & PC & DUTY)".
+    iIntros "(#INV & #MEM & #SPIN & TID & PC & DUTY & #PRM)".
+    iPoseProof (isSpinlock_unfold with "SPIN") as "[#OBL _]".
 
     unfold fn2th. simpl. unfold thread1, Client05Spec.thread1. rred2r. lred2r.
 
+    iRevert "TID PC DUTY".
+    iMod (tpromise_ind with "[] []") as "IH"; cycle 2. done.
+    { iSplit; auto. iExists 3; auto. }
+    iModIntro. iIntros "IH". iModIntro. iIntros "TID PC DUTY".
+
+    iMod (pc_drop _ 1 _ _ 10 with "PC") as "PC". lia.
     iEval (rewrite unfold_iter_eq). rred2r.
     iApply (wpsim_yieldR_gen with "[DUTY] [-]"). auto. iSplitL; done.
     iIntros "DUTY CRED". iModIntro. rred2r.
+    iMod ("IH" with "CRED") as "IH".
     iApply (SCMem_compare_fun_spec with "[] [-]"). instantiate (1:=n). auto. set_solver.
     { simpl. des_ifs. iApply (tgt_interp_as_equiv with "MEM"). iIntros. iSplit.
       { iIntros. simpl. red_tl; simpl. iSplit; [done | iPureIntro; auto]. }
@@ -174,194 +181,134 @@ Section SPEC.
     }
     iIntros (rv) "[%EQ _]". exploit EQ. auto. i; subst. rred2r. iApply wpsim_tauR. rred2r.
     iApply (wpsim_yieldR_gen with "[DUTY] [-]"). auto. iSplitL; done.
-    iIntros "DUTY CRED2". iModIntro. rred2r. iApply wpsim_tauR. rred2r.
+    iIntros "DUTY CRED". iModIntro. rred2r. iApply wpsim_tauR. rred2r.
 
-    iApply (Spinlock_lock_spec_use1 with "[PC DUTY]"). auto.
-    { iEval (red_tl_all; rewrite red_syn_tgt_interp_as; simpl). iFrame. iSplit; [done | iSplit; done]. }
+    iApply (Spinlock_lock_spec with "[] [PC DUTY]"). set_solver.
+    2:{ red_tl_all. rewrite red_syn_tgt_interp_as. iFrame. repeat iSplit; auto. } auto.
     iIntros (_) "POST". iEval (red_tl; simpl) in "POST".
-    iDestruct "POST" as (γu) "POST". iEval (red_tl; simpl) in "POST".
-    iDestruct "POST" as (u) "POST". iEval (red_tl_all; simpl) in "POST".
-    iDestruct "POST" as "(EX & _ & WS & DUTY & PC)". rred2r.
+    iDestruct "POST" as (γs) "POST". iEval (red_tl; simpl) in "POST".
+    iDestruct "POST" as (κu) "POST". iEval (red_tl_all; simpl) in "POST".
+    iDestruct "POST" as "(LW & _ & DUTY & PC)". rred2r.
 
-    iMod (pc_drop _ 1 _ _ 3 with "PC") as "PC". auto.
-    iPoseProof (pc_split _ _ 1 2 with "PC") as "[PC1 PC]".
-    iApply (wpsim_yieldR_gen with "[DUTY PC1] [-]"). auto.
+    iPoseProof (pc_split _ _ 1 with "PC") as "[PC' PC]".
+    iApply (wpsim_yieldR_gen with "[DUTY PC'] [-]"). auto.
     { iSplitL "DUTY"; [done | ]. iApply pcs_cons_fold. iSplitL; done. }
-    iIntros "DUTY CRED3". iModIntro. rred2r.
+    iIntros "DUTY _". iModIntro. rred2r.
 
     iInv "INV" as "CI" "CI_CLOSE".
-    iEval (unfold client05Inv; simpl; red_tl_all; simpl; rewrite red_syn_until_tpromise) in "CI".
-    iDestruct "CI" as "[#OBL UPRM]".
-    iPoseProof (until_tpromise_get_tpromise with "UPRM") as "#PRM".
-    (* Induction point *)
-    iRevert (γu u) "DUTY TID EX WS CI_CLOSE PC".
-    iMod (until_tpromise_ind with "[UPRM] [-]") as "IH"; cycle 2.
-    { done. }
-    { iSplit; done. }
-    iSplit.
-    { iModIntro. iIntros "IH". iModIntro. iIntros "PRE" (γu u) "DUTY TID EX WS CI_CLOSE PC".
-      iEval (simpl; red_tl_all) in "PRE". iDestruct "PRE" as "[PEND PTD]".
-      iApply (SCMem_load_fun_spec with "[PTD]"). auto.
+    iEval (unfold client05Inv; simpl; red_tl_all; simpl) in "CI".
+    iDestruct "CI" as "[[LIVE PTD] | [#SHOT PTD]]".
+    { iApply (SCMem_load_fun_spec with "[PTD]"). auto.
       { pose proof mask_disjoint_N_Client05_state_tgt. set_solver. }
       { iSplitR; done. }
       iIntros (rv) "[%EQ' PTD]"; subst. clear EQ. rred2r. iApply wpsim_tauR. rred2r.
 
-      iPoseProof (pc_split _ _ 1 1 with "PC") as "[PC1 PC]".
-      iApply (wpsim_yieldR_gen with "[DUTY PC1] [-]"). auto.
-      { iSplitL "DUTY"; [done | ]. iApply pcs_cons_fold. iSplitL; done. }
-      iIntros "DUTY CRED".
-
-      iMod (tpromise_progress with "[CRED]") as "[PCk | #DEAD]".
+      iMod (tpromise_progress with "[CRED]") as "[PC' | #SHOT]".
       { iSplitR; done. }
-      2:{ iEval (simpl; red_tl_all) in "DEAD". iDestruct "DEAD" as "[SHOT _]".
-          iExFalso; iApply (OneShots.pending_not_shot with "PEND"). done.
+      2:{ iEval (simpl; red_tl_all) in "SHOT".
+          iExFalso; iApply (OneShots.pending_not_shot with "LIVE"). done.
       }
 
-      iMod ("CI_CLOSE" with "[PEND PTD]") as "_".
-      { unfold client05Inv; simpl; red_tl_all; simpl; rewrite red_syn_until_tpromise. iSplit; [done | ].
-        iApply (until_tpromise_make1 with "[PEND PTD]"). iSplitR. done. simpl; red_tl_all; simpl. iFrame.
+      iDestruct "IH" as "[IH | #SHOT]"; cycle 1.
+      { iEval (simpl; red_tl_all) in "SHOT".
+        iExFalso; iApply (OneShots.pending_not_shot with "LIVE"). done.
       }
-      iModIntro. rred2r. iApply wpsim_tauR. rred2r.
-      iApply (Spinlock_unlock_spec_use1 with "[PC DUTY EX WS]"). auto.
+
+      iMod ("CI_CLOSE" with "[LIVE PTD]") as "_".
+      { unfold client05Inv; simpl; red_tl_all; simpl. iLeft; iFrame. }
+
+      iPoseProof (pc_split _ _ 1 with "PC") as "[PC'' PC]".
+      iApply (wpsim_yieldR_gen with "[DUTY PC''] [-]"). auto.
+      { iSplitL "DUTY"; [done | ]. iApply pcs_cons_fold. iSplitL; done. }
+      iIntros "DUTY _". iModIntro. rred2r. iApply wpsim_tauR. rred2r.
+
+      iPoseProof (pc_split _ _ 1 with "PC") as "[PC'' PC]".
+      iApply (Spinlock_unlock_spec with "[PC'' DUTY LW]"). set_solver.
       { iEval (red_tl_all; rewrite red_syn_tgt_interp_as; simpl). iFrame. iSplitR; [done | iSplitR; [done | ]].
-        iSplitR; [done | iApply pcs_cons_fold; iSplitL; done].
+        iApply pcs_cons_fold; iSplitL; done.
       }
       iIntros (_) "DUTY". iEval (red_tl; simpl) in "DUTY". rred2r. iApply wpsim_tauR.
 
-      iEval (rewrite unfold_iter_eq). rred2r.
-      iApply (wpsim_yieldR_gen with "[DUTY] [-]"). auto. iSplitL; done.
-      iIntros "DUTY CRED". iModIntro. rred2r.
-      iApply (SCMem_compare_fun_spec with "[] [-]"). instantiate (1:=n). auto. set_solver.
-      { simpl. des_ifs. iApply (tgt_interp_as_equiv with "MEM"). iIntros. iSplit.
-        { iIntros. simpl. red_tl; simpl. iSplit; [done | iPureIntro; auto]. }
-        { simpl. red_tl; simpl. iIntros "[? _]". done. }
-      }
-      iIntros (rv) "[%EQ _]". exploit EQ. auto. i; subst. rred2r. iApply wpsim_tauR. rred2r.
-      iApply (wpsim_yieldR_gen with "[DUTY] [-]"). auto. iSplitL; done.
-      iIntros "DUTY CRED2". iModIntro. rred2r. iApply wpsim_tauR. rred2r.
-
-      iApply (Spinlock_lock_spec_use1 with "[PCk DUTY]"). auto.
-      { iEval (red_tl_all; rewrite red_syn_tgt_interp_as; simpl). iFrame. iSplit; [done | iSplit; done]. }
-      iIntros (_) "POST". iEval (red_tl; simpl) in "POST". clear γu u.
-      iDestruct "POST" as (γu) "POST". iEval (red_tl; simpl) in "POST".
-      iDestruct "POST" as (u) "POST". iEval (red_tl_all; simpl) in "POST".
-      iDestruct "POST" as "(EX & _ & WS & DUTY & PC)". rred2r.
-      
-      iMod (pc_drop _ 1 _ _ 3 with "PC") as "PC". auto.
-      iPoseProof (pc_split _ _ 1 2 with "PC") as "[PC1 PC]".
-      iApply (wpsim_yieldR_gen with "[DUTY PC1] [-]"). auto.
-      { iSplitL "DUTY"; [done | ]. iApply pcs_cons_fold. iSplitL; done. }
-      iIntros "DUTY CRED3". iModIntro. rred2r.
-
-      iInv "INV" as "CI" "CI_CLOSE".
-      iEval (unfold client05Inv; simpl; red_tl_all; simpl; rewrite red_syn_until_tpromise) in "CI".
-      iDestruct "CI" as "[_ UPRM]".
-      iMod ("IH" with "[CRED UPRM]") as "IH". iFrame.
-      iApply ("IH" $! γu u with "DUTY TID EX WS CI_CLOSE PC").
+      iApply wpsim_reset. iApply ("IH" with "TID PC' DUTY").
     }
-    {
-      iModIntro. iIntros "#DONE" (γu u) "DUTY TID EX WS CI_CLOSE PC".
-      iEval (unfold t2_write; simpl; red_tl_all; rewrite red_syn_inv) in "DONE".
-      iDestruct "DONE" as "[#SHOT #TINV]".
-      iInv "TINV" as "TI" "TI_CLOSE". iEval (simpl; red_tl_all) in "TI".
-      iApply (SCMem_load_fun_spec with "[TI]"). auto.
-      { pose proof mask_disjoint_N_Client05_N_t2_write; pose proof mask_disjoint_N_Client05_state_tgt;
-          pose proof mask_disjoint_N_t2_write_state_tgt. set_solver.
-      }
+    { iApply (SCMem_load_fun_spec with "[PTD]"). auto.
+      { pose proof mask_disjoint_N_Client05_state_tgt. set_solver. }
       { iSplitR; done. }
       iIntros (rv) "[%EQ' PTD]"; subst. clear EQ. rred2r. iApply wpsim_tauR. rred2r.
 
-      iPoseProof (pc_split _ _ 1 1 with "PC") as "[PC1 PC]".
-      iApply (wpsim_yieldR_gen with "[DUTY PC1] [-]"). auto.
+      iMod ("CI_CLOSE" with "[PTD]") as "_".
+      { unfold client05Inv; simpl; red_tl_all; simpl. iRight; iFrame. done. }
+
+      iPoseProof (pc_split _ _ 1 with "PC") as "[PC'' PC]".
+      iApply (wpsim_yieldR_gen with "[DUTY PC''] [-]"). auto.
       { iSplitL "DUTY"; [done | ]. iApply pcs_cons_fold. iSplitL; done. }
-      iIntros "DUTY CRED".
+      iIntros "DUTY _". iModIntro. rred2r. iApply wpsim_tauR. rred2r.
 
-      iMod ("TI_CLOSE" with "[PTD]") as "_".
-      { simpl; red_tl_all; done. }
-      iMod ("CI_CLOSE" with "[]") as "_".
-      { unfold client05Inv; simpl; red_tl_all; simpl; rewrite red_syn_until_tpromise. iSplit; [done | ].
-        iApply (until_tpromise_make2 with "[]"). iSplitR. done. iModIntro.
-        unfold t2_write; simpl; red_tl_all; simpl; rewrite red_syn_inv. iSplit; done.
-      }
-      iModIntro. rred2r. iApply wpsim_tauR. rred2r.
-
-      iApply (Spinlock_unlock_spec_use1 with "[PC DUTY EX WS]"). auto.
+      iPoseProof (pc_split _ _ 1 with "PC") as "[PC'' PC]".
+      iApply (Spinlock_unlock_spec with "[PC'' DUTY LW]"). set_solver.
       { iEval (red_tl_all; rewrite red_syn_tgt_interp_as; simpl). iFrame. iSplitR; [done | iSplitR; [done | ]].
-        iSplitR; [done | iApply pcs_cons_fold; iSplitL; done].
+        iApply pcs_cons_fold; iSplitL; done.
       }
       iIntros (_) "DUTY". iEval (red_tl; simpl) in "DUTY". rred2r. iApply wpsim_tauR.
 
       iEval (rewrite unfold_iter_eq). rred2r.
       iApply (wpsim_sync_gen with "[DUTY] [-]"). auto. iSplitL; done.
       iIntros "DUTY _". iModIntro. rred2r.
-      iApply (SCMem_compare_fun_spec with "[] [-]"). instantiate (1:=n). auto. set_solver.
-      { simpl. des_ifs. iApply (tgt_interp_as_equiv with "MEM"). iIntros. iSplit.
+
+      iApply (SCMem_compare_fun_spec); auto.
+      { simpl. iApply (tgt_interp_as_equiv with "MEM"). iIntros. iSplit.
         { iIntros. simpl. red_tl; simpl. iSplit; [done | iPureIntro; auto]. }
         { simpl. red_tl; simpl. iIntros "[? _]". done. }
       }
-      iIntros (rv) "[_ %NEQ]". exploit NEQ. auto. i; subst. rred2r. iApply wpsim_tauR. rred2r. lred2r.
-      iApply (wpsim_ret). auto. iModIntro. unfold term_cond. iFrame. iPureIntro; reflexivity.
+      iIntros (rv) "[_ %NEQ]". exploit NEQ. ii. clarify. i; subst.
+      rred2r. iApply wpsim_tauR. rred2r. lred2r. iApply wpsim_ret. auto. iModIntro.
+      iFrame. auto.
     }
-  Unshelve. all: auto.
+  Unshelve. auto.
   Qed.
 
   Lemma Client05_thread2_spec
         tid n
     :
-    ⊢ ⟦(∀ (γw kw γL γe γs : τ{nat, 1+n}),
-           ((⤉ syn_inv n N_Client05 (client05Inv γw kw n))
-              ∗ (syn_tgt_interp_as n sndl (fun m => (s_memory_black m)))
-              ∗ (⤉ isSpinlock n L γL γe kw 4)
-              ∗ (⤉ isSpinlockUse1 n kw γs γL emp 2)
-              ∗ TID(tid)
-              ∗ (⤉ Duty(tid) [(kw, 3, (▿ γw tt) ∗ t2_write n)])
-              ∗ ◇[kw](4, 2)
-              ∗ (⤉ △ γw (1/2)))
-             -∗
-             syn_wpsim (S n) tid ⊤
-             (fun rs rt => (⤉ (syn_term_cond n tid _ rs rt))%S)
-             false false
-             (fn2th Client05Spec.module "thread2" (tt ↑))
-             (fn2th Client05.module "thread2" (tt ↑)))%S, 1+n⟧.
+    ⊢ ⟦(∀ (γw κw γL : τ{nat, 1+n}),
+      ((⤉ syn_inv n N_Client05 (client05Inv n γw))
+        ∗ (syn_tgt_interp_as n sndl (fun m => (s_memory_black m)))
+        ∗ (⤉ isSpinlock spinlockN n κw L γL emp 3 3)
+        ∗ TID(tid)
+        ∗ ◇[κw](3, 1)
+        ∗ (⤉ △ γw (1/2))
+        ∗ (⤉ Duty(tid) [(κw, 2, (▿ γw tt)%S)])
+        ∗ (⤉ -[κw](2)-◇ (▿ γw tt)))
+      -∗
+        syn_wpsim (S n) tid ⊤
+        (fun rs rt => (⤉ (syn_term_cond n tid _ rs rt))%S)
+        false false
+        (fn2th Client05Spec.module "thread2" (tt ↑))
+        (fn2th Client05.module "thread2" (tt ↑)))%S, 1+n⟧.
   Proof.
-    iIntros. red_tl. iIntros "%γw". red_tl. iIntros "%kw".
-    red_tl. iIntros "%γL". red_tl. iIntros "%γe". red_tl. iIntros "%γs".
+    iIntros. red_tl. iIntros "%γw". red_tl. iIntros "%κw". red_tl. iIntros "%γL".
     red_tl_all; simpl. rewrite red_syn_inv; rewrite red_syn_tgt_interp_as; rewrite red_syn_wpsim.
 
-    iIntros "(#INV & #MEM & #SPIN & #SPIN1 & TID & DUTY & PC & PEND)".
+    iIntros "(#INV & #MEM & #SPIN & TID & PC & PEND & DUTY & #PRM)".
 
     unfold fn2th. simpl. unfold thread2, Client05Spec.thread2. rred2r. lred2r.
-    iPoseProof (pc_split _ _ 1 1 with "PC") as "[PC1 PC]".
-    iApply (wpsim_sync with "[DUTY PC1]"). auto. iFrame. iApply pcs_cons_fold; iFrame.
-    iIntros "DUTY CRED".
+    iApply (wpsim_sync with "[DUTY PC]"). auto. iFrame. iApply pcs_cons_fold; iFrame.
+    iIntros "DUTY _".
     rred2r.
     iInv "INV" as "TI" "TI_CLOSE". iEval (simpl; unfold client05Inv; red_tl_all; simpl) in "TI".
-    iDestruct "TI" as "[#OBL UPRM]". iEval (rewrite red_syn_until_tpromise) in "UPRM".
-
-    unfold until_thread_promise. iDestruct "UPRM" as "[#PRM [YET | #DONE]]"; cycle 1.
-    { iEval (simpl; red_tl_all) in "DONE".
-      iDestruct "DONE" as "[SHOT _]"; iExFalso; iApply (OneShots.pending_not_shot with "PEND"); done.
-    }
-    iEval (simpl; red_tl_all) in "YET". iDestruct "YET" as "[PEND2 PTD]".
-    iPoseProof (OneShots.pending_merge _ (1/2) (1/2) with "PEND PEND2") as "PEND". rewrite Qp.half_half.
+    iDestruct "TI" as "[[PEND' PTD] | [#SHOT _]]"; cycle 1.
+    { iExFalso. iApply (OneShots.pending_not_shot with "PEND SHOT"). }
+    
+    iPoseProof (OneShots.pending_merge _ (1/2) (1/2) with "PEND PEND'") as "PEND". rewrite Qp.half_half.
     iMod (OneShots.pending_shot with "PEND") as "#SHOT".
+    iMod (duty_fulfill with "[DUTY]") as "DUTY".
+    { iFrame. simpl; red_tl_all. iSplitR; auto. iPoseProof (unfold_tpromise with "PRM") as "[_ #AO]". auto. }
     iApply (SCMem_store_fun_spec with "[PTD] [-]"). auto.
     { pose proof mask_disjoint_N_Client05_state_tgt; set_solver. }
     { iSplitR; done. }
-    iIntros (rv) "PTD".
-    rred2r. iApply wpsim_tauR. rred2r. lred2r.
-
-    iMod (FUpd_alloc _ _ _ n N_t2_write (D ↦ 1)%S with "[PTD]") as "#CI". auto.
-    { simpl; red_tl_all; auto. }
-
-    iMod (duty_fulfill with "[DUTY]") as "DUTY".
-    { iFrame. simpl; red_tl_all. iSplitR; auto. }
-
-    iMod ("TI_CLOSE" with "[]") as "_".
-    { unfold client05Inv; simpl; red_tl_all; simpl. iSplitR; [done | ]. rewrite red_syn_until_tpromise.
-      iApply (until_tpromise_make2). iSplit; [done | ].
-      iModIntro; simpl; unfold t2_write; red_tl_all; iSplit; done.
-    }
+    iIntros (rv) "PTD". rred2r. iApply wpsim_tauR. rred2r. lred2r.
+    iMod ("TI_CLOSE" with "[PTD]") as "_".
+    { unfold client05Inv; simpl; red_tl_all; simpl. iRight; auto. }
     
     iApply wpsim_ret. auto. iModIntro. unfold term_cond; iFrame; iPureIntro; reflexivity.
   Qed.
@@ -382,9 +329,8 @@ Section SPEC.
 
     Lemma init_sat E (H_TID : tid1 <> tid2) :
       (OwnM (memory_init_resource Client05.gvs))
-        ∗ (OwnM (AuthExcls.rest_ra (gt_dec 0) 0))
         ∗ (OwnM (AuthExcls.rest_ra (gt_dec 0) (0, 0)))
-        ∗ (OwnM (Excls.rest_ra (gt_dec 0) tt))
+        (* ∗ (OwnM (Excls.rest_ra (gt_dec 0) tt)) *)
         ∗
         (WSim.initial_prop
            Client05Spec.module Client05.module
@@ -397,31 +343,32 @@ Section SPEC.
            idx init_ths init_ord)
         ⊢
         =| 1+idx |=(⟦syn_fairI (1+idx), 1+idx⟧)={ E, E }=>
-            (∃ γw kw γL γe γs,
-                (inv idx N_Client05 (client05Inv γw kw idx))
+            (∃ γw κw γL,
+                (inv idx N_Client05 (client05Inv idx γw))
                   ∗ (⟦syn_tgt_interp_as idx sndl (fun m => (s_memory_black m)), 1+idx⟧)
-                  ∗ (⟦isSpinlock idx L γL γe kw 4, idx⟧)
-                  ∗ (⟦isSpinlockUse1 idx kw γs γL emp%S 2, idx⟧)
+                  ∗ (⟦isSpinlock spinlockN idx κw L γL emp%S 3 3, idx⟧)
                   ∗ (own_thread tid1
                       ∗ (⟦Duty(tid1) [], idx⟧)
-                      ∗ ◇[kw](3, 1))
+                      ∗ (◇[κw](2, 1))
+                      ∗ (-[κw](2)-◇ (▿ γw tt : @sProp STT Γ idx)%S))
                   ∗ ((own_thread tid2)
-                      ∗ (⟦Duty(tid2) [(kw, 3, ((▿ γw tt : @sProp STT Γ idx) ∗ t2_write idx)%S)], idx⟧)
-                      ∗ ◇[kw](4, 2) ∗ (△ γw (1/2)))
+                      ∗ (⟦Duty(tid2) [(κw, 2, (▿ γw tt : @sProp STT Γ idx)%S)], idx⟧)
+                      ∗ (◇[κw](3, 1))
+                      ∗ (△ γw (1/2))
+                      ∗ (-[κw](2)-◇ (▿ γw tt : @sProp STT Γ idx)%S))
             ).
     Proof.
-      iIntros "(MEM & REST1 & REST2 & REST & INIT)". rewrite red_syn_fairI.
+      iIntros "(MEM & REST & INIT)". rewrite red_syn_fairI.
       iPoseProof (memory_init_iprop with "MEM") as "[MEM PTS]".
 
-      iMod (alloc_obligation 4 4) as "(%kw & #LO & PC)".
+      iMod (alloc_obligation_fine 3 3) as "(%kw & #LO & PC & PENDING)".
+      iEval (rewrite <- Qp.half_half) in "PENDING".
+      iPoseProof (pending_split _ (1/2) (1/2) with "PENDING") as "(PENDING1 & PENDING2)".
+
       iMod (OneShots.alloc) as "(%γw & LIVE)".
       iEval (rewrite <- Qp.half_half) in "LIVE".
       iPoseProof (OneShots.pending_split _ (1/2) (1/2) with "LIVE") as "(LIVE1 & LIVE2)".
-      iMod (AuthExcls.alloc_gt _ (0) with "[REST1]") as "[REST1 (%γL & BL & WL)]".
-      { iExists 0. done. }
-      iMod (AuthExcls.alloc_gt _ (0, 0) with "[REST2]") as "[REST2 (%γs & BS & WS)]".
-      { iExists 0. done. }
-      iMod (Excls.alloc_gt tt with "[REST]") as "[REST (%γe & EX)]".
+      iMod (AuthExcls.alloc_gt _ (0, 0) with "[REST]") as "[REST (%γl & LB & LW)]".
       { iExists 0. done. }
 
       unfold WSim.initial_prop.
@@ -442,20 +389,18 @@ Section SPEC.
       iPoseProof (natmap_prop_remove_find _ _ _ H with "INIT3") as "[TH2 INIT3]".
       clear H.
 
-      iEval (replace 4 with (2+2) at 2 by lia) in "PC".
-      iPoseProof (pc_split with "PC") as "[PC1 PC2]".
-      iEval (replace 2 with (1+1) at 2 by lia) in "PC2".
-      iPoseProof (pc_split with "PC2") as "[PC2 PC3]".
-      iMod (pc_drop _ 3 _ _ 1 with "PC3") as "PC3". auto.
-      (* iEval (replace 3 with (2+1) at 2 by lia) in "PC3".
-      iPoseProof (pc_split with "PC3") as "[PC3 PC4]". *)
-      iMod (duty_add (v:=idx) with "[DU2 PC2] []") as "DU2".
-      { iSplitL "DU2". instantiate (1:=[]). iApply "DU2". iFrame. }
-      { instantiate (1:=((▿ γw tt : @sProp STT Γ idx) ∗ t2_write idx)%S). simpl. red_tl_all.
-        unfold t2_write. rewrite red_syn_inv. iModIntro. iIntros "#P". auto.
+      iPoseProof (pc_split _ _ 1 with "PC") as "[PC' PC]".
+      iMod (duty_add with "[DU2 PENDING2 PC'] []") as "DU2".
+      { instantiate (4:=[]). iFrame. }
+      { instantiate (1:=(▿ γw tt : @sProp STT Γ idx)%S).
+        iModIntro. simpl; red_tl. iIntros "H". red_tl_all.
+        iPoseProof "H" as "#H". iModIntro; red_tl_all; auto.
       }
-      iPoseProof (duty_tpromise with "DU2") as "#PROM2".
+      iPoseProof (duty_delayed_tpromise with "DU2") as "#DPRM2".
       { ss. eauto. }
+      iMod (activate_tpromise with "DPRM2 PENDING1") as "[#TPRM _]".
+      iPoseProof (pc_split _ _ 1 with "PC") as "[PC' PC]".
+      iMod (pc_drop _ 2 _ _ 1 with "PC'") as "PC'". auto.
 
       iMod (tgt_interp_as_id _ _ (n:=idx) with "[INIT5 MEM]") as "TGT_ST".
       auto.
@@ -473,33 +418,33 @@ Section SPEC.
 
       simpl. unfold SCMem.init_gvars, gvs. ss. des_ifs.
       iDestruct "PTS" as "((PT & _) & (PT2 & _) & _)".
-      iMod (FUpd_alloc _ _ _ idx N_Client05 (client05Inv γw kw idx) with "[PT LIVE1]") as "INV1".
+      iMod (FUpd_alloc _ _ _ idx N_Client05 (client05Inv idx γw) with "[PT LIVE1]") as "INV1".
       lia.
-      { simpl. unfold client05Inv. red_tl_all. rewrite red_syn_until_tpromise. simpl.
-        iSplitR. eauto. iSplitR. auto. simpl. iLeft. red_tl_all. iFrame.
+      { simpl. unfold client05Inv. red_tl_all. iLeft; iFrame.
         ss. clarify.
         Local Transparent SCMem.alloc.
         unfold SCMem.alloc in Heq1. ss; des_ifs. unfold SCMem.alloc in Heq2; ss; des_ifs.
         Local Opaque SCMem.alloc.
       }
-      iMod (FUpd_alloc _ _ _ idx N_Spinlock (spinlockInv idx L γL γe) with "[PT2 BL EX]") as "SI".
+      iMod (FUpd_alloc _ _ _ idx spinlockN (spinlockInv idx kw L γl emp%S) with "[PT2 LB LW]") as "SI".
       lia.
-      { simpl. unfold spinlockInv. red_tl_all. iLeft; iFrame.
+      { simpl. unfold spinlockInv. red_tl_all. iExists 0. red_tl. iExists 0. red_tl_all. iFrame. iLeft. iFrame.
         (* TODO : make lemmas *)
         Local Transparent SCMem.alloc.
         unfold SCMem.alloc in Heq1. ss; des_ifs.
         unfold SCMem.alloc in Heq2; ss; des_ifs.
         Local Opaque SCMem.alloc.
       }
-      iMod (FUpd_alloc _ _ _ idx N_SpinlockUse1 (spinlockUse1 idx kw γs γL emp%S 1)
+      (* iMod (FUpd_alloc _ _ _ idx N_SpinlockUse1 (spinlockUse1 idx kw γl γL emp%S 1)
         with "[WL BS WS]") as "#S1I".
       lia.
       { simpl. unfold spinlockUse1. do 2 (red_tl_all; iExists 0). red_tl_all; simpl.
         iSplitL "BS"; iFrame. iLeft; iFrame.
-      }
-      iModIntro. iExists γw, kw, γL, γe, γs. red_tl_all.
-      rewrite red_syn_tgt_interp_as. unfold isSpinlock, isSpinlockUse1.
-      red_tl_all; rewrite ! red_syn_inv; simpl. iFrame. iSplitR; [done | iSplit; [iPureIntro; lia | done]].
+      } *)
+      iModIntro. iExists γw, kw, γl. red_tl_all.
+      rewrite red_syn_tgt_interp_as. unfold isSpinlock.
+      red_tl_all; rewrite ! red_syn_inv; simpl. repeat iSplit; auto.
+      iFrame. repeat iSplit; auto.
     Unshelve. auto.
     Qed.
 
