src/example/SpinlockSpec0.v
@@ -7,7 +7,7 @@ From Fairness Require Import Spinlock.
 From Fairness Require Import PCM IProp IPM IPropAux.
 From Fairness Require Import IndexedInvariants OpticsInterp SimWeakest.
 From Fairness Require Import TemporalLogic SCMemSpec.
-From Fairness Require Import OneShotsRA AuthExclsRA ExclsRA.
+From Fairness Require Import OneShotsRA AuthExclsRA.
 
 Section SPEC.
 
@@ -26,16 +26,14 @@ Section SPEC.
 
   Context {HasMEMRA: @GRA.inG memRA Γ}.
   Context {HasOneShots : @GRA.inG (OneShots.t unit) Γ}.
-  (* Context {HasAuthExcl : @GRA.inG (AuthExcls.t nat) Γ}. *)
   Context {HasAuthExcl2 : @GRA.inG (AuthExcls.t (nat * nat)) Γ}.
-  Context {HasExcls : @GRA.inG (Excls.t unit) Γ}.
 
-  Ltac red_tl_all := red_tl; red_tl_memra; red_tl_authexcls; red_tl_excls; red_tl_oneshots.
+  Ltac red_tl_all := red_tl; red_tl_memra; red_tl_authexcls; red_tl_oneshots.
 
   Context (spinlockN : namespace) `{DISJ: (↑N_state_tgt :coPset) ## (↑spinlockN : coPset)}.
 
   (** Invariants. *)
-  Definition spinlockInv (n : nat) κs (x : SCMem.val) (γx γl : nat) (P : sProp n)
+  Definition spinlockInv (n : nat) κs (x : SCMem.val) (γl : nat) (P : sProp n)
     : sProp n :=
     (∃ (γκu κu : τ{nat}),
         (● γl (γκu, κu))
@@ -52,35 +50,35 @@ Section SPEC.
   (*          ∨ (⌜l = 1⌝ ∗ (△ γκu 1) ∗ (-[κu](0)-◇ (▿ γκu tt)) ∗ (κu -(0)-◇ κs))) *)
   (*   )%S. *)
 
-  Definition isSpinlock n κs (x : SCMem.val) (γx γl : nat) (P : sProp n) (ℓL μn : nat)
+  Definition isSpinlock n κs (x : SCMem.val) (γl : nat) (P : sProp n) (ℓL μn : nat)
     : sProp n :=
-    (◆[κs, ℓL, μn] ∗ syn_inv n spinlockN (spinlockInv n κs x γx γl P))%S.
+    (◆[κs, ℓL, μn] ∗ syn_inv n spinlockN (spinlockInv n κs x γl P))%S.
 
-  Global Instance isSpinlock_persistent n κs (x : SCMem.val) (γx γl : nat) (P : sProp n) ℓL μn :
-    Persistent (⟦isSpinlock n κs x γx γl P ℓL μn, n⟧).
+  Global Instance isSpinlock_persistent n κs (x : SCMem.val) (γl : nat) (P : sProp n) ℓL μn :
+    Persistent (⟦isSpinlock n κs x γl P ℓL μn, n⟧).
   Proof.
     unfold Persistent. iIntros "H". unfold isSpinlock. red_tl.
     rewrite red_syn_inv. iDestruct "H" as "#H". auto.
   Qed.
 
   Lemma isSpinlock_unfold
-        n κs (x : SCMem.val) (γx γl : nat) (P : sProp n) (ℓL μn : nat)
+        n κs (x : SCMem.val) (γl : nat) (P : sProp n) (ℓL μn : nat)
     :
-    ⟦(isSpinlock n κs x γx γl P ℓL μn), n⟧
-      ⊢ (◆[κs, ℓL, μn] ∗ inv n spinlockN (spinlockInv n κs x γx γl P))%I.
+    ⟦(isSpinlock n κs x γl P ℓL μn), n⟧
+      ⊢ (◆[κs, ℓL, μn] ∗ inv n spinlockN (spinlockInv n κs x γl P))%I.
   Proof.
     unfold isSpinlock. red_tl. rewrite red_syn_inv. iIntros "[A B]". iFrame.
   Qed.
 
   Lemma pass_lock
-        n κs (x : SCMem.val) (γx γl : nat) (P : sProp n) (ℓL μn : nat)
+        n κs (x : SCMem.val) (γl : nat) (P : sProp n) (ℓL μn : nat)
         tid γκu κu ϕ
         ℓl μa γκu' κu'
         E
         (SUB : (↑spinlockN) ⊆ E)
     :
     ⊢
-      (⟦((isSpinlock n κs x γx γl P ℓL μn)
+      (⟦((isSpinlock n κs x γl P ℓL μn)
            ∗ (○ γl (γκu, κu)) ∗ (Duty(tid) ((κu, 0, ▿ γκu tt) :: ϕ))
            ∗ ◇[κs](ℓl, μa)
            ∗ ◆[κu', ℓl, μa] ∗ ⧖[κu', (1/2)] ∗ (△ γκu' 1) ∗ (-[κu'](0)-⧖ (▿ γκu' tt))
@@ -115,15 +113,15 @@ Section SPEC.
     iModIntro. iFrame. auto.
   Qed.
 
-
   Lemma Spinlock_lock_spec
         tid n
     :
-    ⊢ ∀ κs x γx γl (P : sProp n) ℓL μn (ds : list (nat * nat * sProp n)) ℓu μu,
+    ⊢ ∀ κs x γl (P : sProp n) ℓL μn (ds : list (nat * nat * sProp n)) ℓu μu,
+      (⌜0 < ℓu⌝) →
         [@ tid, n, ⊤ @]
           ⧼⟦((syn_tgt_interp_as n sndl (fun m => (s_memory_black m)))
-               ∗ (⤉ isSpinlock n κs x γx γl P ℓL μn)
-               ∗ ◇[κs](1 + ℓu, μu)
+               ∗ (⤉ isSpinlock n κs x γl P ℓL μn)
+               ∗ ◇[κs](ℓu, 1 + μu)
                ∗ (⤉ Duty(tid) ds)
                ∗ ◇{ds@1}(1 + ℓL, μn)
                ∗ ◇{ds@1}(1, 1)
@@ -138,10 +136,78 @@ Section SPEC.
   .
   Proof.
     iIntros (? ? ? ? ? ? ? ? ? ?).
-    iStartTriple. iIntros "PRE POST". unfold Spinlock.lock.
+    iStartTriple. iIntros "PRE POST".
+    iEval (red_tl_all; rewrite red_syn_tgt_interp_as) in "PRE"; simpl.
+    iDestruct "PRE" as "(#MEM & #SPIN & PCs & DUTY & PCS & PCS')".
+    iPoseProof (isSpinlock_unfold with "SPIN") as "[#OBL #INV]". iClear "SPIN".
+    unfold Spinlock.lock.
     (* Preprocess for induction. *)
-  Admitted.
-
+    iMod (ccs_make_fine with "[OBL PCS]") as "CCS". iSplitR. done. instantiate (1:=1). done.
+    iRevert "PCS' PCs DUTY POST". iMod (ccs_ind2 with "[CCS] []") as "IH". done. 2: iApply "IH".
+    iModIntro. iExists 0. iIntros "IH". iModIntro. iIntros "PCS PCs DUTY POST".
+    (* Yield *)
+    iEval (rewrite unfold_iter_eq). rred2r.
+    iApply (wpsim_yieldR2 with "[DUTY PCS]"). auto. auto. iFrame.
+    iIntros "DUTY CRED _". rred2r.
+    (* Open invariant *)
+    iInv "INV" as "SI" "SI_CLOSE".
+    iEval (unfold spinlockInv; simpl; red_tl_all) in "SI".
+    iDestruct "SI" as (γs) "SI". iEval (red_tl) in "SI".
+    iDestruct "SI" as (κu) "SI". iEval (red_tl_all; simpl) in "SI".
+    iDestruct "SI" as "(LB & [(PTX & LW & P) | (PTX & LIVE & #PRM & #LINK)])".
+    { (* Success *)
+      iApply (SCMem_cas_fun_spec with "[PTX] [-]"). auto. set_solver. iFrame.
+      { simpl. iApply (tgt_interp_as_equiv with "MEM"). iIntros. iSplit.
+        { iIntros. simpl. red_tl; simpl. iSplit; [done | iPureIntro; auto]. }
+        { simpl. red_tl; simpl. iIntros "[? _]". done. }
+      }
+      iIntros (rv) "[%u [%H' PTX]]". des_ifs. des; clarify. rred2r. iApply wpsim_tauR. rred2r.
+      (* Allocate unlocking obligation *)
+      iMod OneShots.alloc as "[%γs' LIVE]".
+      iMod (alloc_obligation_fine ℓu (1 + μu)) as "(%κu' & #OBL' & PC & PENDING)".
+      iPoseProof (pc_split _  _ 1 with "PC") as "[PC' PC]".
+      iAssert (#=> ◇[κu'](1, 1))%I with "[PC']" as "> PC'".
+      { destruct (Nat.eq_dec ℓu 1). subst; done.
+        iMod (pc_drop _ 1 _ _ 1 1 with "[PC']") as "PC'". auto. done. done.
+      }
+      iEval (rewrite <- Qp.half_half) in "PENDING".
+      iPoseProof (pending_split with "PENDING") as "[PENDING PENDING']".
+      iMod (duty_add with "[DUTY PC' PENDING] []") as "DUTY". iFrame.
+      { instantiate (1:= (▿ γs' tt)%S). simpl. iModIntro. red_tl_all. iIntros "#H". iModIntro. done. }
+      iPoseProof (duty_delayed_tpromise with "DUTY") as "#DPRM". simpl; left; auto.
+      iMod (activate_tpromise with "DPRM PENDING'") as "[#PRM _]". iClear "DPRM".
+      iMod (AuthExcls.b_w_update _ _ _ (γs', κu') with "LB LW") as "[LB LW]".
+      iMod (link_new_fine _ _ _ _ 0 with "[PCs]") as "#LINK".
+      { iSplitR; cycle 1. iApply "PCs". done. }
+      (* Close the invariant *)
+      iMod ("SI_CLOSE" with "[PTX LIVE LB]") as "_".
+      { iEval (simpl; unfold spinlockInv; red_tl_all). iExists γs'. red_tl. iExists κu'. red_tl_all.
+        iFrame. iRight; iFrame. iSplit; auto.
+      }
+      iApply ("POST" with "[-]").
+      { do 2 (red_tl; iExists _); red_tl_all; iFrame. }
+    }
+    { (* Failure *)
+      iApply (SCMem_cas_fun_spec with "[PTX] [-]"). auto. set_solver. iFrame.
+      { simpl. iApply (tgt_interp_as_equiv with "MEM"). iIntros. iSplit.
+        { iIntros. simpl. red_tl; simpl. iSplit; [done | iPureIntro; auto]. }
+        { simpl. red_tl; simpl. iIntros "[? _]". done. }
+      }
+      iIntros (rv) "[%u [%H' PTX]]". des_ifs. des; clarify. rred2r. iApply wpsim_tauR. rred2r. iApply wpsim_tauR.
+      iMod (tpromise_progress with "[PRM CRED]") as "[PC | #SHOT]". iFrame. done.
+      2:{ iExFalso. iEval (simpl; red_tl_all) in "SHOT". iApply (OneShots.pending_not_shot with "LIVE SHOT"). }
+      iMod (link_amplify with "[LINK PC]") as "PC". iFrame. done. simpl.
+      iMod ("IH" with "PC") as "IH".
+      (* Close the invariant *)
+      iMod ("SI_CLOSE" with "[PTX LIVE LB]") as "_".
+      { iEval (simpl; unfold spinlockInv; red_tl_all). iExists γs. red_tl. iExists κu. red_tl_all.
+        iFrame. iRight; iFrame. iSplit; auto.
+      }
+      iApply wpsim_stutter_mon. instantiate (1:=ps); auto. instantiate (1:=pt); auto.
+      iApply ("IH" with "PCs DUTY POST").
+    }
+  Unshelve. lia.
+  Qed.
   (* Lemma red_syn_Spinlock_lock_spec *)
   (*       tid n *)
   (*       (Es : coPsets) *)
@@ -218,10 +284,10 @@ Section SPEC.
   Lemma Spinlock_unlock_spec
         tid n
     :
-    ⊢ ∀ κs x γx γl (P : sProp n) ℓL μn (ds : list (nat * nat * sProp n)) γκu κu,
+    ⊢ ∀ κs x γl (P : sProp n) ℓL μn (ds : list (nat * nat * sProp n)) γκu κu,
         [@ tid, n, ⊤ @]
           ⧼⟦((syn_tgt_interp_as n sndl (fun m => (s_memory_black m)))
-               ∗ (⤉ isSpinlock n κs x γx γl P ℓL μn)
+               ∗ (⤉ isSpinlock n κs x γl P ℓL μn)
                ∗ (⤉ ○ γl (γκu, κu))
                ∗ (⤉ P)
                ∗ (⤉ Duty(tid) ((κu, 0, ▿ γκu tt) :: ds))
@@ -231,10 +297,37 @@ Section SPEC.
             ⧼rv, ⟦((⤉ Duty(tid) ds))%S, 1+n⟧⧽
   .
   Proof.
-    iIntros (? ? ? ? ? ? ? ? ? ?).
-    iStartTriple. iIntros "PRE POST". unfold Spinlock.unlock.
+    iIntros (? ? ? ? ? ? ? ? ?).
+    iStartTriple. iIntros "PRE POST".
     (* Preprocess. *)
-  Admitted.
+    iEval (red_tl_all; rewrite red_syn_tgt_interp_as) in "PRE"; simpl.
+    iDestruct "PRE" as "(#MEM & #SPIN & LW & P & DUTY & PCS)".
+    iPoseProof (isSpinlock_unfold with "SPIN") as "[#OBL #INV]". iClear "SPIN".
+    unfold Spinlock.unlock.
+    (* Yield *)
+    rred2r. iApply (wpsim_yieldR with "[DUTY PCS]"). auto. iFrame. done.
+    iIntros "DUTY _". rred2r.
+    (* Open invariant *)
+    iInv "INV" as "SI" "SI_CLOSE".
+    iEval (unfold spinlockInv; simpl; red_tl_all) in "SI".
+    iDestruct "SI" as (γs') "SI". iEval (red_tl) in "SI".
+    iDestruct "SI" as (κu') "SI". iEval (red_tl_all; simpl) in "SI".
+    iDestruct "SI" as "(LB & [(PTX & LW' & _) | (PTX & LIVE & #PRM & #LINK)])".
+    { iExFalso. iApply (AuthExcls.w_w_false with "LW LW'"). }
+    iPoseProof (AuthExcls.b_w_eq with "LB LW") as "%EQ"; clarify.
+    (* Store *)
+    iApply (SCMem_store_fun_spec with "[PTX] [-]"). auto. set_solver.
+    { iFrame. done. }
+    iIntros (rv) "PTX". rred2r. iApply wpsim_tauR. rred2r.
+    (* Close invariant *)
+    iPoseProof (unfold_tpromise with "PRM") as "[_ #AO]".
+    iMod (OneShots.pending_shot _ tt with "LIVE") as "#SHOT".
+    iMod (duty_fulfill with "[DUTY]") as "DUTY".
+    { iFrame. simpl; red_tl_all. iSplit; done. }
+    iMod ("SI_CLOSE" with "[PTX LB LW P]") as "_".
+    { iEval (simpl; unfold spinlockInv; red_tl_all). do 2 (iExists _; red_tl_all). iFrame. iLeft; iFrame. }
+    iApply "POST". red_tl. done.
+  Qed.
 
   (* Lemma red_syn_Spinlock_unlock_spec *)
   (*       tid n *)
